Proof stronger equation system rationality

src/Rational/RationalTerm.v
@@ -1,3 +1,6 @@
+From Stdlib Require Import List.
+Import ListNotations.
+
 Require Import Unification.
 
 CoInductive inf_term : Set :=
@@ -15,6 +18,13 @@ end.
 
 Lemma inf_term_step_prop t : t = inf_term_step t.
 Proof. intros. destruct t; reflexivity. Qed.
+
+Fixpoint term_to_inf (t : term) : inf_term :=
+match t with
+| Var x => InfVar x
+| Cst c => InfCst c
+| Con f l r => InfCon f (term_to_inf l) (term_to_inf r)
+end.
 
 Inductive path : Set :=
 | Here : path
@@ -64,6 +74,20 @@ Proof.
   * eexists. constructor. constructor. reflexivity.
   * apply H1 in H6. destruct H6 as [ r' [ H1_1 H1_2 ] ]. exists r'. constructor; auto. constructor. auto.
   * apply H2 in H6. destruct H6 as [ r' [ H2_1 H2_2 ] ]. exists r'. constructor; auto. constructor. auto.
+Qed.
+
+Lemma inf_term_eq_conl n1 n2 l1 l2 r1 r2 (H : inf_term_eq (InfCon n1 l1 r1) (InfCon n2 l2 r2))
+                     : inf_term_eq l1 l2.
+Proof.
+  intros p l1' Hp. destruct (H (Left p) l1') as [ r [ H1 H2 ] ]. constructor. auto.
+  exists r. good_inversion H1. constructor; auto.
+Qed.
+
+Lemma inf_term_eq_conr n1 n2 l1 l2 r1 r2 (H : inf_term_eq (InfCon n1 l1 r1) (InfCon n2 l2 r2))
+                     : inf_term_eq r1 r2.
+Proof.
+  intros p r1' Hp. destruct (H (Right p) r1') as [ r [ H1 H2 ] ]. constructor. auto.
+  exists r. good_inversion H1. constructor; auto.
 Qed.
 
 Instance inf_term_eq_refl : RelationClasses.Reflexive inf_term_eq.
@@ -134,10 +158,216 @@ Proof.
       + exists cr'. constructor; auto. constructor. auto.
 Qed.
 
+Lemma inf_path_to_eq p l1 l2 r1 r2 (H1 : inf_term_eq l1 l2) (H2 : inf_term_eq r1 r2)
+                     (H3 : inf_path_to l1 p r1)
+                   : exists t, inf_path_to l2 p t /\ inf_term_eq t r2.
+Proof.
+  revert l2 r2 H1 H2. induction H3; intros.
+  * exists l2. constructor. constructor. etransitivity. symmetry. eauto. auto.
+  * destruct l2 as [ | | f' l' r' ].
+    - edestruct (H1 Here). constructor. destruct H. good_inversion H. inversion H0.
+    - edestruct (H1 Here). constructor. destruct H. good_inversion H. inversion H0.
+    - edestruct IHinf_path_to as [ t' [ IH1 IH2 ] ]. eapply inf_term_eq_conl. eauto. eauto.
+      exists t'. constructor; auto. constructor. auto.
+  * destruct l2 as [ | | f' l' r' ].
+    - edestruct (H1 Here). constructor. destruct H. good_inversion H. inversion H0.
+    - edestruct (H1 Here). constructor. destruct H. good_inversion H. inversion H0.
+    - edestruct IHinf_path_to as [ t' [ IH1 IH2 ] ]. eapply inf_term_eq_conr. eauto. eauto.
+      exists t'. constructor; auto. constructor. auto.
+Qed.
+
 Instance inf_term_eq_equiv : RelationClasses.Equivalence inf_term_eq :=
   RelationClasses.Build_Equivalence _ _ _ _.
 
 Definition inf_subterm (l r : inf_term) := exists p, inf_path_to l p r.
 
+Instance inf_subterm_refl : RelationClasses.Reflexive inf_subterm.
+Proof. intro. exists Here. constructor. Qed.
+
+Instance inf_subterm_trans : RelationClasses.Transitive inf_subterm.
+Proof.
+  intros a b c H1. destruct H1 as [ p H1 ]. revert c. induction H1; intros. auto.
+  * edestruct IHinf_path_to as [ q IH ]. eauto. exists (Left q). constructor. auto.
+  * edestruct IHinf_path_to as [ q IH ]. eauto. exists (Right q). constructor. auto.
+Qed.
+
+Lemma inf_subterm_eq l1 l2 r1 r2 (H1 : inf_term_eq l1 l2) (H2 : inf_term_eq r1 r2)
+                     (H3 : inf_subterm l1 r1)
+                   : exists t, inf_subterm l2 t /\ inf_term_eq t r2.
+Proof.
+  destruct H3 as [ p H ]. eapply inf_path_to_eq in H; eauto.
+  destruct H as [ t [ H3 H4 ] ]. exists t. constructor; auto. exists p. auto.
+Qed.
+
 Definition is_rational_term (t : inf_term) :=
-  exists ts, forall l, inf_subterm t l -> exists r, inf_term_eq l r /\ List.In r ts.
+  exists ts, forall l, inf_subterm t l -> Exists (inf_term_eq l) ts.
+
+Lemma is_rational_eq t1 t2 (H1 : inf_term_eq t1 t2) (H2 : is_rational_term t1) : is_rational_term t2.
+Proof.
+  destruct H2 as [ ts H2 ]. exists ts. intros. eapply inf_subterm_eq in H.
+  destruct H as [ t [ H3 H4 ] ]. apply H2 in H3. clear H2. apply Exists_exists in H3.
+  destruct H3 as [ t' [ H2 H3 ] ]. apply Exists_exists. exists t'. constructor. auto.
+  etransitivity. symmetry. apply H4. auto. symmetry. auto. reflexivity.
+Qed.
+
+Lemma inf_subterm_rational l r (H1 : is_rational_term l) (H2 : inf_subterm l r) : is_rational_term r.
+Proof. destruct H1 as [ ts H1 ]. exists ts. intros. apply H1. transitivity r; auto. Qed.
+
+Fixpoint term_subterms (t : term) : list term :=
+match t with
+| Var _ => [t]
+| Cst _ => [t]
+| Con f l r => t :: term_subterms l ++ term_subterms r
+end.
+
+Lemma term_subterms_self t : In t (term_subterms t).
+Proof. induction t; left; auto. Qed.
+
+Lemma term_subterms_incl t1 t2 (H : In t1 (term_subterms t2)) : incl (term_subterms t1) (term_subterms t2).
+Proof.
+  induction t2; simpl in H.
+  * destruct H. subst. apply incl_refl. inversion H.
+  * destruct H. subst. apply incl_refl. inversion H.
+  * destruct H. subst. apply incl_refl. apply in_app_or in H. simpl. apply incl_tl. destruct H.
+    - apply incl_appl. auto.
+    - apply incl_appr. auto.
+Qed.
+
+Lemma term_to_inf_rational t : is_rational_term (term_to_inf t).
+Proof.
+  exists (map term_to_inf (term_subterms t)). intros. destruct H as [ p H ].
+  remember (term_to_inf t) as t'. revert t Heqt'. induction H; intros.
+  * subst. apply Exists_map. apply Exists_exists. exists t0. constructor.
+    apply term_subterms_self. reflexivity.
+  * destruct t0 as [ | | f' l' r' ]; good_inversion Heqt'.
+    apply Exists_map. simpl. apply Exists_cons_tl. apply Exists_app. left. apply Exists_map.
+    apply IHinf_path_to. auto.
+  * destruct t0 as [ | | f' l' r' ]; good_inversion Heqt'.
+    apply Exists_map. simpl. apply Exists_cons_tl. apply Exists_app. right. apply Exists_map.
+    apply IHinf_path_to. auto.
+Qed.
+
+Definition inf_subst : Set := list (name * inf_term).
+
+Definition inf_subst_empty : inf_subst := [].
+
+Definition inf_subst_singleton (x : name) (t : inf_term) : inf_subst := [(x, t)].
+
+Fixpoint inf_subst_dom (s : inf_subst) : var_set :=
+match s with
+| [] => var_set_empty
+| (x, _) :: s => var_set_add x (inf_subst_dom s)
+end.
+
+Fixpoint inf_image (s : inf_subst) (x : name) : option inf_term :=
+match s with
+| [] => None
+| (y, t) :: s => if name_eq_dec x y then Some t else inf_image s x
+end.
+
+Lemma inf_image_dom s x : (exists t, inf_image s x = Some t) <-> In x (inf_subst_dom s).
+Proof.
+  induction s as [ | [ y t ] s ]; simpl.
+  * constructor; intro. destruct H as [ t H ]. inversion H. inversion H.
+  * destruct (name_eq_dec x y).
+    - constructor; intro. apply ListSet.set_add_intro2. auto. eexists. reflexivity.
+    - constructor; intro. apply ListSet.set_add_intro1. apply IHs. auto.
+      apply ListSet.set_add_elim in H. destruct H. contradiction. apply IHs. auto.
+Qed.
+
+Definition is_rational_subst (s : inf_subst) :=
+  exists ts, forall x t, inf_image s x = Some t ->
+    forall l, inf_subterm t l -> Exists (inf_term_eq l) (ts x).
+
+Fact inf_image_rational s x t (H1 : is_rational_subst s) (H2 : inf_image s x = Some t) : is_rational_term t.
+Proof. destruct H1 as [ ts H1 ]. exists (ts x). apply H1. auto. Qed.
+
+CoFixpoint inf_subst_apply (s : inf_subst) (t : inf_term) : inf_term :=
+match t with
+| InfVar x => match inf_image s x with None => t | Some t' => t' end
+| InfCst _ => t
+| InfCon f l r => InfCon f (inf_subst_apply s l) (inf_subst_apply s r)
+end.
+
+Lemma inf_subst_apply_eq_node s t1 t2 (H : inf_term_eq_node t1 t2)
+                       : inf_term_eq_node (inf_subst_apply s t1) (inf_subst_apply s t2).
+Proof. destruct t1; destruct t2; good_inversion H; reflexivity. Qed.
+
+Lemma inf_subst_apply_eq s t1 t2 (H : inf_term_eq t1 t2)
+                       : inf_term_eq (inf_subst_apply s t1) (inf_subst_apply s t2).
+Proof.
+  intros p t1' Hp. remember (inf_subst_apply s t1) as t. revert t1 t2 H Heqt.
+  induction Hp; intros.
+  * subst. eexists. constructor. constructor.
+    specialize (H Here t1). destruct H as [ t2' [ H1 H2 ] ]. constructor.
+    good_inversion H1. apply inf_subst_apply_eq_node. auto.
+  * rewrite inf_term_step_prop in Heqt. destruct t1; good_inversion Heqt.
+    - edestruct (H Here) as [ t2' [ H2 H3 ] ]. constructor. good_inversion H2.
+      destruct t2'; good_inversion H3. clear H. remember (inf_image s n0) as t'.
+      destruct t' as [ [ | | f' l' r' ] | ]; good_inversion H1.
+      exists t. constructor. rewrite inf_term_step_prop at 1. simpl. rewrite <- Heqt'.
+      constructor. auto. reflexivity.
+    - edestruct (H Here) as [ t2' [ H1 H2 ] ]. constructor. good_inversion H1.
+      destruct t2'; good_inversion H2. specialize (IHHp t1_1 t2'1).
+      destruct IHHp as [ r' [ IH1 IH2 ] ]; auto. eapply inf_term_eq_conl. eauto.
+      exists r'. constructor; auto. rewrite inf_term_step_prop at 1. constructor. auto.
+  * rewrite inf_term_step_prop in Heqt. destruct t1; good_inversion Heqt.
+    - edestruct (H Here) as [ t2' [ H2 H3 ] ]. constructor. good_inversion H2.
+      destruct t2'; good_inversion H3. clear H. remember (inf_image s n0) as t'.
+      destruct t' as [ [ | | f' l' r' ] | ]; good_inversion H1.
+      exists t. constructor. rewrite inf_term_step_prop at 1. simpl. rewrite <- Heqt'.
+      constructor. auto. reflexivity.
+    - edestruct (H Here) as [ t2' [ H1 H2 ] ]. constructor. good_inversion H1.
+      destruct t2'; good_inversion H2. specialize (IHHp t1_2 t2'2).
+      destruct IHHp as [ r' [ IH1 IH2 ] ]; auto. eapply inf_term_eq_conr. eauto.
+      exists r'. constructor; auto. rewrite inf_term_step_prop at 1. constructor. auto.
+Qed.
+
+Lemma inf_subst_apply_subterm s l r (H : inf_subterm (inf_subst_apply s l) r)
+                            : (exists t, inf_subterm l t /\ inf_term_eq (inf_subst_apply s t) r)
+                           \/ (exists x t, inf_subterm l (InfVar x)
+                                        /\ inf_image s x = Some t
+                                        /\ inf_subterm t r).
+Proof.
+  destruct H as [ p H ]. remember (inf_subst_apply s l) as l'. revert l Heql'. induction H; intros.
+  * left. exists l. constructor. reflexivity. subst. reflexivity.
+  * destruct l0 as [ x | | f' l' r' ]; rewrite inf_term_step_prop in Heql'; good_inversion Heql'.
+    - remember (inf_image s x) as x'. destruct x' as [ x' | ]; good_inversion H1.
+      destruct x'; good_inversion H2. right. exists x. exists (InfCon n x'1 x'2).
+      constructor. reflexivity. constructor. auto. exists (Left p). constructor. auto.
+    - specialize (IHinf_path_to _ eq_refl). destruct IHinf_path_to as [ IH | IH ].
+      + destruct IH as [ t' [ IH1 IH2 ] ]. left. exists t'. constructor; auto.
+        destruct IH1 as [ q IH1 ]. exists (Left q). constructor. auto.
+      + destruct IH as [ x [ t' [ IH1 IH2 ] ] ]. right. exists x. exists t'. constructor; auto.
+        destruct IH1 as [ q IH1 ]. exists (Left q). constructor. auto.
+  * destruct l0 as [ x | | f' l' r' ]; rewrite inf_term_step_prop in Heql'; good_inversion Heql'.
+    - remember (inf_image s x) as x'. destruct x' as [ x' | ]; good_inversion H1.
+      destruct x'; good_inversion H2. right. exists x. exists (InfCon n x'1 x'2).
+      constructor. reflexivity. constructor. auto. exists (Right p). constructor. auto.
+    - specialize (IHinf_path_to _ eq_refl). destruct IHinf_path_to as [ IH | IH ].
+      + destruct IH as [ t' [ IH1 IH2 ] ]. left. exists t'. constructor; auto.
+        destruct IH1 as [ q IH1 ]. exists (Right q). constructor. auto.
+      + destruct IH as [ x [ t' [ IH1 IH2 ] ] ]. right. exists x. exists t'. constructor; auto.
+        destruct IH1 as [ q IH1 ]. exists (Right q). constructor. auto.
+Qed.
+
+Lemma inf_subst_apply_rational s t (H1 : is_rational_subst s) (H2 : is_rational_term t)
+                             : is_rational_term (inf_subst_apply s t).
+Proof.
+  destruct H1 as [ tsf H1 ]. destruct H2 as [ ts H2 ].
+  exists (map (inf_subst_apply s) ts ++ flat_map tsf (inf_subst_dom s)). intros.
+  apply inf_subst_apply_subterm in H. destruct H.
+  * destruct H as [ t' [ H3 H4 ] ]. apply H2 in H3. apply Exists_exists in H3.
+    destruct H3 as [ r [ H3 H5 ] ]. apply Exists_app. left. apply Exists_map. apply Exists_exists.
+    exists r. constructor. auto. etransitivity. symmetry. eauto. apply inf_subst_apply_eq. auto.
+  * destruct H as [ x [ t' [ H3 [ H4 H5 ] ] ] ]. apply Exists_app. right. apply Exists_flat_map.
+    apply Exists_exists. exists x. constructor. apply inf_image_dom. eexists. eauto.
+    eapply H1. eauto. auto.
+Qed.
+
+Definition inf_unifier (s : inf_subst) (t1 t2 : inf_term) : Prop :=
+  inf_term_eq (inf_subst_apply s t1) (inf_subst_apply s t2).
+
+Definition inf_subst_more_general (m s : inf_subst) : Prop :=
+  exists (s' : inf_subst), forall (t : inf_term),
+    inf_term_eq (inf_subst_apply s t) (inf_subst_apply s' (inf_subst_apply m t)).
